src/cddl/pulse/CDDL.Pulse.Serialize.Gen.MapGroup.ZeroOrMore.Aux2.Lemma2.fsti
@@ -1,0 +1,36 @@
+module CDDL.Pulse.Serialize.Gen.MapGroup.ZeroOrMore.Aux2.Lemma2
+include CDDL.Pulse.Serialize.Gen.MapGroup.ZeroOrMore.Aux2.Invariant
+
+module S = Pulse.Lib.Slice
+module U8 = FStar.UInt8
+module SZ = FStar.SizeT
+module U64 = FStar.UInt64
+module Map = CDDL.Spec.Map
+
+val impl_serialize_map_zero_or_more_iterator_gen_invariant0_insert
+  (#pe: cbor_parser)
+  (#minl: cbor_min_length pe)
+  (#maxl: cbor_max_length pe)
+  (#tkey: Type)
+  (#tvalue: Type)
+  (p: cbor_map_parser minl maxl)
+  (em': bool)
+  (out: S.slice U8.t)
+  (vout': Seq.seq U8.t)
+  (size2': SZ.t)
+  (count count': U64.t)
+  (m: cbor_map)
+  (vk vv: cbor)
+  (v': Map.t tkey (list tvalue))
+: Lemma
+  (requires
+    Seq.length vout' == SZ.v (S.len out) /\
+    SZ.v size2' <= Seq.length vout' /\
+    cbor_serialize_map_insert_post p m vk vv true (Seq.slice vout' 0 (SZ.v size2')) /\
+    cbor_map_length m == U64.v count /\
+    U64.v count' == U64.v count + 1 /\
+    (em' == true <==> v' == Map.empty _ _)
+  )
+  (ensures
+    impl_serialize_map_zero_or_more_iterator_gen_invariant p em' out vout' size2' count' (cbor_map_union m (cbor_map_singleton vk vv)) v' true
+  )
